\documentclass[Dissertation.tex]{subfiles} 
\begin{document}

\chapter{Extra Derivations}
\label{chp:ExtraDer}

\section{Spherical Bessel Derivatives}
\label{sec:SphBess}

%\begin{figure}[H]
	%\centering
	%\includegraphics[width=3.5in]{Untitled-2}
	%\caption{Mathematica}
	%\label{fig:Untitled-2}
%\end{figure}


From Abramowitz and Stegun \cite[p.437]{Abramowitz1965},
\begin{subequations}
\begin{align}
j_\ell(z) &= z^{-1} \left[ P(\ell+\tfrac{1}{2}, z ) \sin(z-\tfrac{1}{2}\ell\pi) + Q(\ell+\tfrac{1}{2},z) \cos(z-\tfrac{1}{2}\ell\pi) \right] \\
n_\ell(z) &= (-1)^{\ell+1} z^{-1} \left[ P(\ell+\tfrac{1}{2}, z ) \cos(z+\tfrac{1}{2}\ell\pi) - Q(\ell+\tfrac{1}{2},z) \sin(z+\tfrac{1}{2}\ell\pi) \right].
\end{align}
\end{subequations}
where
\begin{subequations}
\begin{align}
P(\ell+\tfrac{1}{2}, z) &= 1 - \frac{\Factorial{\ell+2}}{\Factorial{2} \GammaFunc{\ell-1}} (2z)^{-2} + \ldots \\
Q(\ell+\tfrac{1}{2}, z) &= \frac{\Factorial{\ell+1}}{\Factorial{1} \GammaFunc{\ell}} (2z)^{-1} - \frac{\Factorial{n+3}}{\Factorial{3} \GammaFunc{\ell-2}} (2z)^{-3} + \ldots
\end{align}
\end{subequations}
Using \emph{Mathematica} with these expansions, we get
\begin{subequations}
\begin{align}
\label{eq:SphBesExpan}
j_\ell(z) &= \frac{\sin(z - \tfrac{1}{2}\ell\pi)}{z} + \ldots \\
n_\ell(z) &= \frac{(-1)^{\ell+1} \cos(z + \tfrac{1}{2}\ell\pi)}{z} + \ldots
\end{align}
\end{subequations}
and
\begin{subequations}
\begin{align}
\label{eq:SphBesExpanDer}
{j_\ell}^\prime(z) &= \frac{\cos(z - \tfrac{1}{2}\ell\pi)}{z} + \ldots \\
{n_\ell}^\prime(z) &= \frac{(-1)^{\ell+2} \sin(z + \tfrac{1}{2}\ell\pi)}{z} + \ldots
\end{align}
\end{subequations}

In a more general format than that of Abramowitz and Stegun \cite[p.73]{Abramowitz1965},
\beq
\cos \left(z-\frac{\ell \pi}{2} \right) = \begin{cases} (-1)^{\ell/2} \cos z & \mbox{if } \ell \mbox{ is even} \\ 
(-1)^{(\ell-1)/2} \sin z & \mbox{if } \ell \mbox{ is odd} \end{cases} 
\eeq
and
\beq
\sin \left(z-\frac{\ell \pi}{2} \right) = \begin{cases} (-1)^{\ell/2} \sin z & \mbox{if } \ell \mbox{ is even} \\ 
(-1)^{(\ell+1)/2} \cos z & \mbox{if } \ell \mbox{ is odd} \end{cases} .
\eeq
Also,
\beq
\cos \left(z+\frac{\ell \pi}{2} \right) = \begin{cases} (-1)^{\ell/2} \cos z & \mbox{if } \ell \mbox{ is even} \\ 
(-1)^{(\ell+1)/2} \sin z & \mbox{if } \ell \mbox{ is odd} \end{cases} 
\eeq
and
\beq
\sin \left(z+\frac{\ell \pi}{2} \right) = \begin{cases} (-1)^{\ell/2} \sin z & \mbox{if } \ell \mbox{ is even} \\ 
(-1)^{(\ell-1)/2} \cos z & \mbox{if } \ell \mbox{ is odd} \end{cases} .
\eeq
Using these with \cref{eq:SphBesExpan,eq:SphBesExpanDer}, we see that to first order, there is a relationship between these functions and their derivatives given by
\begin{subequations}
\begin{align}
\label{eq:SphBesDerRel}
{j_\ell}^\prime(z) &\approx -n_\ell(z) \\
{n_\ell}^\prime(z) &\approx j_\ell(z).
\end{align}
\end{subequations}



\section{\texorpdfstring{$_2F_1$}{Hypergeometric} Identity}
\label{sec:Hypergeometric}

The backwards recursion relation for the hypergeometric function is given in Refs. \cite{Drake1995} and \cite{Frolov2003} as
\beq
\label{eq:HyperIdentity}
_2F_1(1,a;c;z) = 1 + \left( \frac{a}{c} \right) z \,\,_2F_1(1,a+1;c+1;z).
\eeq

From Abramowitz and Stegun \cite{Abramowitz1965}, the definition of the hypergeometric function is given by
\beq
\label{eq:HyperDef}
_2F_1(\alpha,\beta;\gamma;z) = 1 + \sum_{n=1}^{\infty} \frac{(\alpha)_n \cdot (\beta)_n}{(\gamma)_n} \frac{z^n}{n!},
\eeq
where $(x)_n$ is the Pochhammer symbol given by \cite{Abramowitz1965}
\beq
\label{eq:PochhammerDef}
(x)_n \equiv \frac{\Gamma(x+n)}{\Gamma(x)} = x(x+1) \cdots  (x+n-1)
\eeq
with $(x)_0 = 1$.  A special case is $(x)_1 = n!$, where $n!$ is the factorial.

Using the above definition of the Pochhammer symbol, we can easily see that
\beq
\label{eq:PochPlus1}
(x+1)_n = \frac{(x+n)}{(x)} \cdot (x)_n = \frac{(x)_{n+1}}{x}.
\eeq

From \ref{eq:HyperDef} and \ref{eq:PochPlus1}, 
\begin{align}
\nonumber _2F_1(1,a+1;c+1;z) &= 1 + \sum_{n=1}^{\infty} \frac{(1)_n \cdot (a+1)_n}{(c+1)_n} \frac{z^n}{n!} = 1 + \sum_{n=1}^{\infty} \frac{(a+1)_n}{(c+1)_n} z^n \\
&= 1 + \left(\frac{c}{a}\right) \sum_{n=1}^{\infty} \frac{(a)_{n+1}}{(c)_{n+1}} z^n = 1 + \left(\frac{c}{a}\right) \sum_{n=2}^{\infty} \frac{(a)_n}{(c)_n} z^{n-1}.
\end{align}
Multiplying by $\left(\frac{c}{a}\right) z$, we now have
\beq
\label{eq:Hyper1}
\left(\frac{c}{a}\right) z _2F_1(1,a+1;c+1;z) = \left(\frac{c}{a}\right) z + \sum_{n=2}^{\infty} \frac{(a)_n}{(c)_n} z^n = \sum_{n=1}^{\infty} \frac{(a)_n}{(c)_n} z^n.
\eeq

From the definition in equation \ref{eq:HyperDef},
\beq
\label{eq:Hyper2}
_2F_1(1,a;c;z) = 1 + \sum_{n=1}^{\infty} \frac{(a)_n}{(c)_n} z^n,
\eeq
which, when combined with equation \ref{eq:Hyper1}, gives the final result of
\beq
_2F_1(1,a;c;z) = 1 + \left( \frac{a}{c} \right) z \,\,_2F_1(1,a+1;c+1;z).
\eeq


\section{Shielding Function}
\label{sec:ShieldingFunc}

\todoi{Give how C acts like S with shielding function}





\biblio
\end{document}